container/coq/pointer/Layer12/Spec.v
@@ -30,19 +30,8 @@ Section Layer12_Spec.
   Definition total_root_rtt_refcount_loop295_rank (v_0: Ptr) (v__011: Z) (v_indvars_iv: Z) (v_wide_trip_count: Z) : Z :=
     v_wide_trip_count.
 
-  Definition find_lock_unused_granule_spec (v_0: Z) (v_1: Z) (st: RData) : (option (Ptr * RData)) :=
-    None.
-
-  Definition ptr_is_err_spec (v_0: Ptr) (st: RData) : (option (bool * RData)) :=
-    if (((int_to_ptr 18446744073709547520).(pbase)) =s ("status"))
-    then (
-      if ((v_0.(pbase)) <>s ("status"))
-      then (Some (false, st))
-      else (Some (((v_0.(poffset)) >? (((int_to_ptr 18446744073709547520).(poffset)))), st)))
-    else (Some ((((ptr_to_int v_0) - (18446744073709547520)) >? (0)), st)).
-
-  Definition ptr_status_spec (v_0: Ptr) (st: RData) : (option (Z * RData)) :=
-    (Some ((0 - ((ptr_to_int v_0))), st)).
+  Definition measurement_finish_spec (v_0: Ptr) (v_1: Ptr) (st: RData) : (option RData) :=
+    (Some st).
 
 End Layer12_Spec.
 
@@ -53,6 +42,4 @@ End Layer12_Spec.
 #[global] Hint Unfold copy_gic_state_to_ns_loop59_rank: spec.
 #[global] Hint Unfold copy_gic_state_from_ns_loop48_rank: spec.
 #[global] Hint Unfold total_root_rtt_refcount_loop295_rank: spec.
-#[global] Hint Unfold find_lock_unused_granule_spec: spec.
-#[global] Hint Unfold ptr_is_err_spec: spec.
-#[global] Hint Unfold ptr_status_spec: spec.
+#[global] Hint Unfold measurement_finish_spec: spec.
