container/coq/pointer/Layer13/Spec.v
@@ -62,7 +62,33 @@ Section Layer13_Spec.
       when st_2 == ((spinlock_release_spec (mkPtr "granules" ((test_PA v_0).(meta_granule_offset))) st_1));
       (Some ((pack_struct_return_code_para (make_return_code_para 1)), st_2))).
 
+  Definition smc_realm_activate_spec (v_0: Z) (st: RData) : (option (Z * RData)) :=
+    when st_1 == ((spinlock_acquire_spec (mkPtr "granules" ((test_PA v_0).(meta_granule_offset))) st));
+    if (((((((st_1.(share)).(globals)).(g_granules)) @ (((test_PA v_0).(meta_granule_offset)) / (16))).(e_state_s_granule)) - (2)) =? (0))
+    then (
+      rely ((((((test_PA v_0).(meta_granule_offset)) mod (16)) = (0)) /\ ((((test_PA v_0).(meta_granule_offset)) >= (0)))));
+      rely (((("granule_data" = ("granule_data")) /\ ((((test_PA v_0).(meta_granule_offset)) >= (0)))) /\ (((((test_PA v_0).(meta_granule_offset)) mod (4096)) = (0)))));
+      rely (((((((st_1.(share)).(granule_data)) @ (((test_PA v_0).(meta_granule_offset)) / (4096))).(g_granule_state)) - (GRANULE_STATE_RD)) = (0)));
+      if ((((((st_1.(share)).(granule_data)) @ (((test_PA v_0).(meta_granule_offset)) / (4096))).(g_rd)).(e_state_s_rd)) =? (0))
+      then (
+        when st_6 == (
+            (granule_unlock_spec
+              (mkPtr "granules" ((test_PA v_0).(meta_granule_offset)))
+              (st_1.[share].[granule_data] :<
+                (((st_1.(share)).(granule_data)) #
+                  (((test_PA v_0).(meta_granule_offset)) / (4096)) ==
+                  ((((st_1.(share)).(granule_data)) @ (((test_PA v_0).(meta_granule_offset)) / (4096))).[g_norm] :<
+                    (((((st_1.(share)).(granule_data)) @ (((test_PA v_0).(meta_granule_offset)) / (4096))).(g_norm)) # (((test_PA v_0).(meta_granule_offset)) mod (4096)) == 1))))));
+        (Some (0, st_6)))
+      else (
+        when st_5 == ((granule_unlock_spec (mkPtr "granules" ((test_PA v_0).(meta_granule_offset))) st_1));
+        (Some ((pack_struct_return_code_para (make_return_code_para 5)), st_5))))
+    else (
+      when st_2 == ((spinlock_release_spec (mkPtr "granules" ((test_PA v_0).(meta_granule_offset))) st_1));
+      (Some ((pack_struct_return_code_para (make_return_code_para 1)), st_2))).
+
 End Layer13_Spec.
 
 #[global] Hint Unfold find_lock_unused_granule_spec_abs: spec.
 #[global] Hint Unfold smc_rec_destroy_spec: spec.
+#[global] Hint Unfold smc_realm_activate_spec: spec.
