container/coq/pointer/Layer10/Layer.v
@@ -9,7 +9,6 @@ Require Import Layer3.Spec.
 Require Import Layer4.Spec.
 Require Import Layer5.Spec.
 Require Import Layer6.Spec.
-Require Import Layer7.Spec.
 Require Import Layer8.Spec.
 
 Local Open Scope string_scope.
@@ -71,6 +70,7 @@ Section Layer10_Layer.
           :: ("find_lock_granule", prim find_lock_granule_spec)
           :: ("find_lock_two_granules", prim find_lock_two_granules_spec)
           :: ("g_refcount", prim g_refcount_spec)
+          :: ("get_rd_state_locked", prim get_rd_state_locked_spec)
           :: ("gic_restore_state", prim gic_restore_state_spec)
           :: ("granule_addr", prim granule_addr_spec)
           :: ("granule_lock", prim granule_lock_spec)
@@ -78,7 +78,6 @@ Section Layer10_Layer.
           :: ("granule_memzero", prim granule_memzero_spec)
           :: ("granule_memzero_mapped", prim granule_memzero_mapped_spec)
           :: ("granule_pa_to_va", prim granule_pa_to_va_spec)
-          :: ("granule_refcount_read_acquire", prim granule_refcount_read_acquire_spec)
           :: ("granule_set_state", prim granule_set_state_spec)
           :: ("granule_unlock", prim granule_unlock_spec)
           :: ("granule_unlock_transition", prim granule_unlock_transition_spec)
