container/coq/pointer/Layer5/set_rd_state/LowSpec.v
@@ -1,4 +1,3 @@
-Require Import Bottom.Spec.
 Require Import Code.
 Require Import CommonDeps.
 Require Import DataTypes.
@@ -13,8 +12,8 @@ Section Layer5_set_rd_state_LowSpec.
 
   Definition set_rd_state_spec_low (v_0: Ptr) (v_1: Z) (st: RData) : (option RData) :=
     rely (((((((st.(share)).(granule_data)) @ ((v_0.(poffset)) / (4096))).(g_granule_state)) - (GRANULE_STATE_RD)) = (0)));
-    rely (((v_0.(pbase)) = ("granule_data")));
-    when st_0 == ((store_RData 64 (mkPtr (v_0.(pbase)) (v_0.(poffset))) v_1 st));
+    rely (((((v_0.(pbase)) = ("granule_data")) /\ (((v_0.(poffset)) >= (0)))) /\ ((((v_0.(poffset)) mod (4096)) = (0)))));
+    when st_0 == ((store_RData_granule_data 64 (ptr_offset v_0 0) v_1 st));
     (Some st_0).
 
 End Layer5_set_rd_state_LowSpec.
